ObjectModel.thy
@@ -38,25 +38,39 @@ fun mapEnrollmentToValList :: "Enrollment list \<Rightarrow> val list" where
 "mapEnrollmentToValList [] = []" |
 "mapEnrollmentToValList (e#es) = (VEnrollment e)#(mapEnrollmentToValList es)"
 
-fun equalVal :: "val \<Rightarrow> val \<Rightarrow> bool" where
-"equalVal (VInt i1) (VInt i2) = (i1 = i2)" |
-"equalVal (VBool b1) (VBool b2) = (b1 \<longleftrightarrow> b2)" |
-"equalVal (VString s1) (VString s2) = (s1 = s2)" |
-"equalVal (VPerson p1) (VPerson p2) = (p1 = p2)" |
-"equalVal (VList []) (VList []) = True" |
-"equalVal (VList (v1#v1s)) (VList (v2#v2s)) = 
-(if (equalVal v1 v2) then (equalVal (VList v1s) (VList v2s)) else False)"
+fun equalVal :: "val \<Rightarrow> val \<Rightarrow> bool"
+and equalValList :: "val list \<Rightarrow> val list \<Rightarrow> bool"
+where
+"equalValList Nil Nil = True"
+| "equalValList Nil e2 = False"
+| "equalValList e1 Nil = False"
+| "equalValList (e1#e1s) (e2#e2s) = (if (equalVal e1 e2) 
+then (equalValList e1s e2s) else False)"
+| "equalVal (VInt i1) (VInt i2) = (i1 = i2)"
+| "equalVal (VBool b1) (VBool b2) = (b1 \<longleftrightarrow> b2)" 
+| "equalVal (VString s1) (VString s2) = (s1 = s2)" 
+| "equalVal (VPerson p1) (VPerson p2) = (p1 = p2)" 
+| "equalVal (VList v1s) (VList v2s) = equalValList v1s v2s"
 
-fun greaterThanVal :: "val \<Rightarrow> val \<Rightarrow> bool" where
-"greaterThanVal (VInt i1) (VInt i2) = (i1 > i2)" |
-"greaterThanVal (VList []) (VList []) = True" |
-"greaterThanVal (VList (v1#v1s)) (VList (v2#v2s)) = 
-(if (greaterThanVal v1 v2) then (greaterThanVal (VList v1s) (VList v2s)) else False)"
+fun greaterThanVal :: "val \<Rightarrow> val \<Rightarrow> bool" 
+and greaterThanValList :: "val list \<Rightarrow> val list \<Rightarrow> bool"
+where
+"greaterThanValList Nil Nil = False"
+| "greaterThanValList Nil e2 = False"
+| "greaterThanValList e1 Nil = False"
+| "greaterThanValList (e1#e1s) (e2#e2s) = (if (greaterThanVal e1 e2) 
+then (greaterThanValList e1s e2s) else False)"
+| "greaterThanVal (VInt i1) (VInt i2) = (i1 > i2)" 
+| "greaterThanVal (VList e1s) (VList e2s) = greaterThanValList e1s e2s"
 
-fun andVal :: "val \<Rightarrow> val \<Rightarrow> bool" where
+fun andVal :: "val \<Rightarrow> val \<Rightarrow> bool"
+and andValList :: "val list \<Rightarrow> val list \<Rightarrow> bool" where
 "andVal (VBool b1) (VBool b2) = (b1 \<and> b2)"
-| "andVal (VList []) (VList []) = True" 
-| "andVal (VList (v1#v1s)) (VList (v2#v2s)) = ((andVal v1 v2) \<and> (andVal (VList v1s) (VList v2s)))"
+| "andVal (VList v1s) (VList v2s) = andValList v1s v2s"
+| "andValList Nil Nil = False"
+| "andValList Nil v2s = False"
+| "andValList e1s Nil = False"
+| "andValList (e1#e1s) (e2#e2s) = ((andVal e1 e2) \<and> (andValList e1s e2s))"
 
 fun countValList :: "val list \<Rightarrow> int" where 
 "countValList [] = 0" |
@@ -67,22 +81,25 @@ fun appendList :: "val \<Rightarrow> val \<Rightarrow> val" where
 "appendList v VNULL = VList [v]" |
 "appendList v (VList vs) = VList (v#vs)"
 
-appendList VEnrollment vs = Cons Vernol (VList vs)
-appendList (VList v) vs vs2 = cons (Vlist v) appendList (vs, vs2_)
-
 fun sizeValList :: "val list\<Rightarrow> nat" where
 "sizeValList [] = 0" |
 "sizeValList (x#xs) = Suc (sizeValList xs)"
 
 fun sizeVal :: "val \<Rightarrow> nat" where
 "sizeVal VNULL = 0" |
-"sizeVal (VList []) = 0" |
-"sizeVal (VList (x#xs)) = Suc (sizeVal (VList xs))"
+"sizeVal (VList vs) = sizeValList vs"
+
+fun isEmptyValList :: "val list \<Rightarrow> bool" where
+"isEmptyValList v = (sizeValList v = 0)"
 
 fun isEmptyVal :: "val \<Rightarrow> bool" where
-"isEmptyVal v = (sizeVal v = 0)"
+"isEmptyVal (VList vs) = isEmptyValList vs"
 
-fun isTrue :: "val \<Rightarrow> bool" where
-"isTrue (VList [VBool (True)]) = True"
+fun isTrueValList :: "val list\<Rightarrow> bool" where
+"isTrueValList [VBool True] = True"
+
+fun isTrueVal :: "val \<Rightarrow> bool" where
+"isTrueVal (VBool True) = True"
+| "isTrueVal (VList vs) = isTrueValList vs"
 
 end
